concurrency/scache/rwlock/CacheHandle.i.dfy
@@ -11,26 +11,30 @@ module CacheHandle {
   import CacheResources
   import opened NativeTypes
 
+  datatype PageHandle = PageHandle(
+      data_ptr: Ptr,
+      disk_addr: int64)
+
   datatype Key = Key(
       data_ptr: Ptrs.Ptr,
-      idx_cell: Cell<int64>,
+      idx_cell: Cell<PageHandle>,
       ghost cache_idx: nat)
 
   glinear datatype Handle =
     | CacheEmptyHandle(
         ghost key: Key,
         glinear cache_empty: CacheResources.CacheEmpty,
-        glinear idx: CellContents<int64>,
+        glinear idx: CellContents<PageHandle>,
         glinear data: PointsToArray<byte>)
     | CacheReadingHandle(
         ghost key: Key,
         glinear cache_reading: CacheResources.CacheReading,
-        glinear idx: CellContents<int64>,
+        glinear idx: CellContents<PageHandle>,
         glinear data: PointsToArray<byte>)
     | CacheEntryHandle(
         ghost key: Key,
         glinear cache_entry: CacheResources.CacheEntry,
-        glinear idx: CellContents<int64>,
+        glinear idx: CellContents<PageHandle>,
         glinear data: PointsToArray<byte>)
   {
     predicate is_handle(key: Key)
@@ -39,18 +43,19 @@ module CacheHandle {
       && this.idx.cell == key.idx_cell
       && this.data.ptr == key.data_ptr
       && |this.data.s| == 4096
-      && 0 <= this.idx.v as int < NUM_DISK_PAGES as int
+      && 0 <= this.idx.v.disk_addr as int < NUM_DISK_PAGES as int
+      && this.idx.v.data_ptr == key.data_ptr
 
       && (this.CacheEmptyHandle? ==>
         && this.cache_empty.cache_idx == key.cache_idx
       )
       && (this.CacheReadingHandle? ==>
         && this.cache_reading.cache_idx == key.cache_idx
-        && this.cache_reading.disk_idx == this.idx.v as int
+        && this.cache_reading.disk_idx == this.idx.v.disk_addr as int
       )
       && (this.CacheEntryHandle? ==>
         && this.cache_entry.cache_idx == key.cache_idx
-        && this.cache_entry.disk_idx == this.idx.v as int
+        && this.cache_entry.disk_idx == this.idx.v.disk_addr as int
         && this.cache_entry.data == this.data.s
       )
     }
